{-# OPTIONS --without-K #-}
module HoTT where

open import Universes public

open import Agda.Builtin.IO using (IO)
open import Agda.Builtin.Unit using (âŠ¤)
open import Agda.Builtin.String using (String)

postulate putStrLn : String â†’ IO âŠ¤
{-# FOREIGN GHC import qualified Data.Text as T #-}
{-# COMPILE GHC putStrLn = putStrLn . T.unpack #-}

main : IO âŠ¤
main = putStrLn "Hello world!"

variable
 ğ“¤ ğ“¥ ğ“¦ ğ“£ : Universe

{- | ğŸ˜
-}
data ğŸ˜ : ğ“¤â‚€â€ŠÌ‡ where

ğŸ˜-induction : (A : ğŸ˜ â†’ ğ“¤â€ŠÌ‡) â†’ (x : ğŸ˜) â†’ A x
ğŸ˜-induction A ()

is-empty : ğ“¤â€ŠÌ‡ â†’ ğ“¤â€ŠÌ‡
is-empty X = X â†’ ğŸ˜

{- | ğŸ™
-}
data ğŸ™ : ğ“¤â‚€â€ŠÌ‡ where
 â‹† : ğŸ™

ğŸ™-induction : (A : ğŸ™ â†’ ğ“¤â€ŠÌ‡) â†’ A â‹† â†’ (x : ğŸ™) â†’ A x
ğŸ™-induction A a â‹† = a

ğŸ™-recursion : (A : ğ“¤â€ŠÌ‡) â†’ A â†’ ğŸ™ â†’ A
ğŸ™-recursion A = ğŸ™-induction (Î» _ â†’ A)

{- | _+_
-}
data _+_ {ğ“¤ ğ“¥} (X : ğ“¤â€ŠÌ‡) (Y : ğ“¥â€ŠÌ‡) : ğ“¤ âŠ” ğ“¥â€ŠÌ‡ where
 inl : X â†’ X + Y
 inr : Y â†’ X + Y

+-induction
 : {X : ğ“¤â€ŠÌ‡} {Y : ğ“¥â€ŠÌ‡} (A : X + Y â†’ ğ“¦â€ŠÌ‡)
 â†’ ((x : X) â†’ A (inl x))
 â†’ ((y : Y) â†’ A (inr y))
 â†’ (z : X + Y)
 â†’ A z
+-induction A f g (inl l) = f l
+-induction A f g (inr r) = g r

+-recursion
 : {X : ğ“¤â€ŠÌ‡} {Y : ğ“¥â€ŠÌ‡} {A : ğ“¦â€ŠÌ‡}
 â†’ (X â†’ A)
 â†’ (Y â†’ A)
 â†’ X + Y
 â†’ A
+-recursion {ğ“¤} {ğ“¥} {ğ“¦} {X} {Y} {A} = +-induction (Î» _ â†’ A)

{- | ğŸš
-}
ğŸš : ğ“¤â‚€â€ŠÌ‡
ğŸš = ğŸ™ + ğŸ™

ğŸš-induction
 : (A : ğŸš â†’ ğ“¤â€ŠÌ‡)
 â†’ A (inl â‹†)
 â†’ A (inr â‹†)
 â†’ (n : ğŸš)
 â†’ A n
ğŸš-induction A aâ‚€ aâ‚ = +-induction A
 (ğŸ™-induction (Î» (x : ğŸ™) â†’ A (inl x)) aâ‚€)
 (ğŸ™-induction (Î» (y : ğŸ™) â†’ A (inr y)) aâ‚)

{- | Î£
-}
record Î£ {ğ“¤ ğ“¥} {X : ğ“¤â€ŠÌ‡} (Y : X â†’ ğ“¥â€ŠÌ‡) : ğ“¤ âŠ” ğ“¥â€ŠÌ‡ where
  constructor
   _,_
  field
   x : X
   y : Y x

-Î£ : {ğ“¤ ğ“¥ : Universe} (X : ğ“¤â€ŠÌ‡) (Y : X â†’ ğ“¥â€ŠÌ‡) â†’ ğ“¤ âŠ” ğ“¥â€ŠÌ‡
-Î£ X Y = Î£ Y

syntax -Î£ X (Î» x â†’ y) = Î£ x ê‰ X , y

Î£-induction
 : {X : ğ“¤â€ŠÌ‡} {Y : X â†’ ğ“¥â€ŠÌ‡} {A : Î£ Y â†’ ğ“¦â€ŠÌ‡}
 â†’ ((x : X) â†’ (y : Y x) â†’ A (x , y))
 â†’ ((x , y) : Î£ Y)
 â†’ A (x , y)
Î£-induction g (x , y) = g x y

uncurry = Î£-induction

curry
 : {X : ğ“¤â€ŠÌ‡} {Y : X â†’ ğ“¥â€ŠÌ‡} {A : Î£ Y â†’ ğ“¦â€ŠÌ‡}
 â†’ (((x , y) : Î£ Y) â†’ A (x , y))
 â†’ ((x : X) (y : Y x) â†’ A (x , y))
curry f x y = f (x , y)

Î£-recursion : ğ“¤â€ŠÌ‡ â†’ ğ“¥â€ŠÌ‡ â†’ ğ“¤ âŠ” ğ“¥â€ŠÌ‡
Î£-recursion X Y = Î£ x ê‰ X , Y

_Ã—_ = Î£-recursion

{- | Î 
-}
Î  : {X : ğ“¤â€ŠÌ‡} (A : X â†’ ğ“¥â€ŠÌ‡) â†’ ğ“¤ âŠ” ğ“¥â€ŠÌ‡
Î  {ğ“¤} {ğ“¥} {X} A = (x : X) â†’ A x

-Î  : {ğ“¤ ğ“¥ : Universe} (X : ğ“¤â€ŠÌ‡) (Y : X â†’ ğ“¥â€ŠÌ‡) â†’ ğ“¤ âŠ” ğ“¥â€ŠÌ‡
-Î  X Y = Î  Y

syntax -Î  A (Î» x â†’ b) = Î  x ê‰ A , b

{- | Functions
-}
_âˆ˜_
 : {X : ğ“¤â€ŠÌ‡} {Y : ğ“¥â€ŠÌ‡} {Z : Y â†’ ğ“¦â€ŠÌ‡}
 â†’ ((y : Y) â†’ Z y)
 â†’ (f : X â†’ Y)
 â†’ ((x : X) â†’ Z (f x))
g âˆ˜ f = Î» x â†’ g (f x)

domain
 : {X : ğ“¤â€ŠÌ‡} {Y : ğ“¥â€ŠÌ‡}
 â†’ (X â†’ Y)
 â†’ ğ“¤â€ŠÌ‡
domain {ğ“¤} {ğ“¥} {X} {Y} f = X

codomain
 : {X : ğ“¤â€ŠÌ‡} {Y : ğ“¥â€ŠÌ‡}
 â†’ (X â†’ Y)
 â†’ ğ“¥â€ŠÌ‡
codomain {ğ“¤} {ğ“¥} {X} {Y} f = Y

type-of : {X : ğ“¤â€ŠÌ‡} â†’ X â†’ ğ“¤â€ŠÌ‡
type-of {ğ“¤} {X} x = X

id : (X : ğ“¤â€ŠÌ‡) â†’ X â†’ X
id X x = x

{- | Id
-}
data Id {ğ“¤} (X : ğ“¤â€ŠÌ‡) : X â†’ X â†’ ğ“¤â€ŠÌ‡ where
 refl : (x : X) â†’ Id X x x

_==_ : {X : ğ“¤â€ŠÌ‡} â†’ X â†’ X â†’ ğ“¤â€ŠÌ‡
x == y = Id _ x y

==-induction
 : (X : ğ“¤â€ŠÌ‡) (A : (x y : X) â†’ Id X x y â†’ ğ“¥â€ŠÌ‡)
 â†’ ((x : X) â†’ A x x (refl x))
 â†’ (x y : X) (p : x == y)
 â†’ A x y p
==-induction X A f x x (refl x) = f x

ğ• = ==-induction

id-transitivity
 : {X : ğ“¤â€ŠÌ‡} {x y z : X}
 â†’ Id X x y
 â†’ Id X y z
 â†’ Id X x z
id-transitivity (refl xy) (refl yz) = refl xz
 where
  xz = xy

reverse-id : {X : ğ“¤â€ŠÌ‡} {x y : X} â†’ Id X x y â†’ Id X y x
reverse-id (refl xy) = refl yx
 where yx = xy

{- | List
-}
data List (A : ğ“¤â€ŠÌ‡) : ğ“¤â€ŠÌ‡ where
 [] : List A
 _âˆ·_ : A â†’ List A â†’ List A

infix 50 _==_
infixr 50 _,_
infixr 30 _Ã—_
infixr 20 _+_
infixl 70 _âˆ˜_
infix   0 Id

-- not exactly correct
-- pullback :
-- (A B C : ğ“¤â€ŠÌ‡) â†’
-- (f : A â†’ C) â†’ (g : B â†’ C) â†’ (a : A) â†’ (b : B) â†’ (f(a) == g(b))
-- pullback A B C f g a b = refl (f (a))

-- infix   0 _âˆ¼_
-- infix   0 _â‰¡_
-- infix  10 _â‡”_
-- infixl 30 _âˆ™_
-- infixr  0 _â‰¡âŸ¨_âŸ©_
-- infix   1 _âˆ
-- infix  40 _â»Â¹
-- infix  10 _â—_
-- infixr  0 _â—âŸ¨_âŸ©_
-- infix   1 _â—€
-- infix  10 _â‰ƒ_
-- infixl 30 _â—_
-- infixr  0 _â‰ƒâŸ¨_âŸ©_
-- infix   1 _â– 
-- infix  40 _âˆˆ_
-- infix  30 _[_,_]
-- infixr -1 -Î£
-- infixr -1 -Î 
-- infixr -1 -âˆƒ!
