{-# OPTIONS --without-K #-}
module NaturalNumbers where

open import Universes public

data ğŸ™ : ğ“¤â‚€ Ì‡  where
 â‹† : ğŸ™

data ğŸ˜ : ğ“¤â‚€ Ì‡ where

variable
 ğ“¤ ğ“¥ ğ“¦ ğ“£ : Universe

data â„• : ğ“¤â‚€ Ì‡ where
 zero : â„•
 succ : â„• â†’ â„•

â„•-induction
 : {A : â„• â†’ ğ“¤â€ŠÌ‡}
 â†’ A zero
 â†’ ((n : â„•) â†’ A n â†’ A (succ n))
 â†’ (n : â„•)
 â†’ A n
â„•-induction aâ‚€ f zero = aâ‚€
â„•-induction aâ‚€ f (succ n) = f n (â„•-induction aâ‚€ f n)

â„•-recursion
 : {X : ğ“¤â€ŠÌ‡}
 â†’ X
 â†’ (â„• â†’ X â†’ X)
 â†’ â„•
 â†’ X
â„•-recursion = â„•-induction

â„•-iteration
 : {X : ğ“¤â€ŠÌ‡}
 â†’ X
 â†’ (X â†’ X)
 â†’ â„•
 â†’ X
â„•-iteration x f = â„•-recursion x (Î» _ â†’ f)

â„•-induction'
 : (A : â„• â†’ ğ“¤â€ŠÌ‡)
 â†’ A zero
 â†’ ((n : â„•) â†’ A n â†’ A (succ n))
 â†’ (n : â„•)
 â†’ A n
â„•-induction' A aâ‚€ f = h
 where
  h : (n : â„•) â†’ A n
  h zero = aâ‚€
  h (succ n) = f n (h n)

â„•-recursion'
 : (X : ğ“¤â€ŠÌ‡)
 â†’ X
 â†’ (â„• â†’ X â†’ X)
 â†’ â„•
 â†’ X
â„•-recursion' X = â„•-induction' (Î» _ â†’ X)

â„•-iteration'
 : (X : ğ“¤â€ŠÌ‡)
 â†’ X
 â†’ (X â†’ X)
 â†’ â„•
 â†’ X
â„•-iteration' X x f = â„•-recursion' X x (Î» _ x â†’ f x)

module Arithmetic where
 _+_  _Ã—_ : â„• â†’ â„• â†’ â„•

 x + zero   = x
 x + succ y = succ (x + y)

 x Ã— zero   = zero
 x Ã— succ y = x + x Ã— y

 infixl 20 _+_
 infixl 21 _Ã—_

module Arithmetic' where
 _+_  _Ã—_ : â„• â†’ â„• â†’ â„•

--  x + y = â„•-recursion x h y
--   where
--    h : â„• â†’ â„• â†’ â„•
--    h x zero = x
--    h x (succ y) = y

 x + y = â„•-iteration x succ y

 x Ã— y = â„•-iteration zero (x +_) y

 infixl 20 _+_
 infixl 21 _Ã—_

module â„•-order where
 _â‰¤_ _â‰¥_ : â„• â†’ â„• â†’ ğ“¤â‚€â€ŠÌ‡

 zero â‰¤ y = ğŸ™
 succ x â‰¤ zero = ğŸ˜
 succ x â‰¤ succ y = x â‰¤ y

 x â‰¥ y = x â‰¤ y

 infix 10 _â‰¤_
 infix 10 _â‰¥_

{-
module â„•-order' where
 _â‰¤_ _â‰¥_ : â„• â†’ â„• â†’ ğ“¤â‚€

 x â‰¤ y = (â„•-induction {â„• â†’ â„• â†’ ğ“¤â€ŠÌ‡} aâ‚€ f x) y
  where
   aâ‚€ : â„• â†’ ğ“¤â€ŠÌ‡
   aâ‚€ y = ğŸ™
   f  (n : â„•) â†’ A n â†’ A (succ n)
   f zero aâ‚™ y = ğŸ™
   f (succ x) aâ‚™ zero = ğŸ˜
   f (succ x) aâ‚™ (succ y) = f x aâ‚™ y

 infix 10 _â‰¤_
 infix 10 _â‰¥_
 -}


{- TODO:
Exercise. After learning Î£ and _ï¼_ explained below, prove that

x â‰¤ y if and only if Î£ z ê‰ â„• , x + z ï¼ y.

Later, after learning univalence prove that in this case this implies

(x â‰¤ y) ï¼ Î£ z ê‰ â„• , x + z ï¼ y.
-}
